code/experimental/P256/Hacl.Spec.ECDSA.fst
@@ -13,21 +13,24 @@ let prime = prime_p256_order
 let nat_prime = (n: nat {n < prime})
 
 
-let ith_bit (k:lbytes 32) (i:nat{i < 256}) : uint64 =
+let ith_bit (k:lbytes 32) (i:nat{i < 256}) : (t: uint64 {uint_v t == 0 \/ uint_v t == 1}) =
   let q = i / 8 in let r = size (i % 8) in
+  admit();
   to_u64 ((index k q >>. r) &. u8 1)
 
 let ( *% ) a b = (a * b) % prime
 
 
-val _exp_step0: p: nat_prime -> q: nat_prime -> tuple2 nat_prime nat_prime
+val _exp_step0: p: nat_prime -> q: nat_prime -> 
+  Tot (t: tuple2 nat_prime nat_prime {let t0, t1 = t in t0 == (p * p) % prime_p256_order /\ t1 == (p * q) % prime_p256_order})
 
 let _exp_step0 r0 r1 = 
   let r1 = r0 *% r1 in 
   let r0 = r0 *% r0 in 
   r0, r1
 
-val _exp_step1: p: nat_prime -> q: nat_prime -> tuple2 nat_prime nat_prime 
+val _exp_step1: p: nat_prime -> q: nat_prime -> 
+  Tot (t: tuple2 nat_prime nat_prime {let t0, t1 = t in t0 == (p * q) % prime_p256_order /\ t1 == (q * q) % prime_p256_order})
 
 let _exp_step1 r0 r1 = 
   let r0 = r0 *% r1 in 
@@ -69,17 +72,19 @@ val lemma_swaped_steps: p: nat_prime -> q: nat_prime ->
 
 let lemma_swaped_steps p q = ()
 
+open Lib.RawIntTypes 
 
-val _exp_step: k:  lseq uint8 32 ->  i: nat{i < 256} ->  (tuple2 nat_prime nat_prime) -> Tot (r: tuple2 nat_prime nat_prime)
+val _exp_step: k:  lseq uint8 32 ->  i: nat{i < 256} -> tuple2 nat_prime nat_prime ->
+  Tot (t: tuple2 nat_prime nat_prime)
 
 let _exp_step k i (p, q) = 
   let bit = 255 - i in 
   let bit = ith_bit k bit in 
-  let open Lib.RawIntTypes in 
   if uint_to_nat bit = 0 then 
       _exp_step0 p q 
   else _exp_step1 p q  
 
+#reset-options "--z3refresh --z3rlimit 300"
 
 val _exponent_spec: k: lseq uint8 32  -> tuple2 nat_prime nat_prime -> Tot (tuple2 nat_prime nat_prime)
 
@@ -112,9 +117,32 @@ let prime_p256_order_seq: lseq uint8 32 =
   assert_norm (List.Tot.length prime_p256_order_list == 32);
   of_list prime_p256_order_list
 
+open Hacl.Spec.P256.Definitions
 
-val exponent_spec: a: nat_prime -> Tot nat_prime
+val exponent_spec: a: nat_prime -> Tot (r: nat_prime {r = pow a (prime_p256_order - 2) % prime_p256_order})
 
 let exponent_spec a = 
-    let a0, _ = _exponent_spec prime_p256_order_inverse_seq (1, a) in 
+    admit();
+    let a0, _ = _exponent_spec prime_p256_order_inverse_seq (1, a) in
     a0
+
+val power_distributivity_2: a: nat -> b: nat -> c: pos -> 
+  Lemma (pow (a * b) c == pow a c * pow b c)
+
+let rec power_distributivity_2 a b c = 
+  match c with 
+  |0 -> ()
+  |1 -> ()
+  | _ ->
+    let open FStar.Tactics in 
+    let open FStar.Tactics.Canon in
+    power_distributivity_2 a b (c - 1);
+    assert(pow (a * b) (c - 1) == pow a (c - 1) * pow b (c - 1));
+    assert(pow (a * b) (c - 1) * pow (a * b) 1 == pow a (c - 1) * pow b (c - 1) * pow (a * b) 1);
+    
+    assert(pow (a * b) (c - 1) * pow (a * b) 1 == pow (a * b) c);
+    assert(pow (a * b) 1 == a * b);
+    assert(pow a (c - 1) * pow b (c - 1) * pow (a * b) 1 == pow a (c - 1) * pow b (c - 1) * a * b);
+    assert_by_tactic (pow a (c - 1) * pow b (c - 1) * a * b == (pow a c * pow b c)) canon;
+    assert(pow a (c - 1) * pow b (c - 1) * pow (a * b) 1 == (pow a c * pow b c));
+    assert(pow a c * pow b c == pow (a * b) c)
